
\subsection{FST and DFA}
% --------------------------------------------------

Combine FST $M$ with DFA $M'$ to test the translated string.
An FST combined with a DFA is a DFA.
Notice that an FST does not have a language; rather than procedures such as DFAs, it instead describes
a function.

\begin{theorem}[]\ \\
    \label{thm:translation_of_DFA}
    $
    \forall \text{\upshape FST} F = \lst{Q_F,\Sigma,\Gamma,\delta_F,s_F},   \\
    \phantom{\forall} \text{\upshape DFA} D = \lst{Q_D,\Gamma,\delta_D,s_D,F_D},  \\
    \exists \text{\upshape DFA} M = \lst{Q,\Sigma,\delta,s,F}
    \text{ s.t.\ }
    $
    \[
        L(M) = f_M^{-1} \( L(M_D) \) \text{ meaning }
        L(M) = \set{ w \in \Sigma^* \mid f_M(w) \in L(M_D) }.
    \]
\end{theorem}

\begin{proof}[Proof of \autoref{thm:translation_of_DFA}]
    \begin{align*}
        \text{Let }
        & Q = Q_F \times Q_D,  \\
        & S = (s_F,s_D),       \\
        & F = Q_F \times F_D,  \\
        & \delta \colon Q \times \Sigma \mapsto Q \text{ s.t.\ } \\
        & \delta((q_F,q_D),a) = \big( q_F', \delta_D^*(q_D,w) \big)
        \text{ where } (q_F',w) = \delta_F(q_F,a).
    \end{align*}
\end{proof}

\subsection{Composing FSTs}
% --------------------------------------------------

\begin{theorem}[FSTs are Composable]
    \label{thm:composable_FST}
    \begin{align*}
        & \forall \text{\upshape FST} M_1 = \lst{Q_1,\Sigma,\Gamma,\delta_1,s_1},
                                      M_2 = \lst{Q_2,\Gamma,\Delta,\delta_2,s_2}, \\
        & \exists \text{\upshape FST} M = M_2 \circ M_1
        \text{ s.t.\ } f_M = f_{M_2} \circ f_{M_1}.
    \end{align*}
\end{theorem}

\begin{proof}[Proof of \autoref{thm:composable_FST}]
    $
    \text{Let } M = (Q, \Sigma, \Delta, \delta, s)
    \text{ where } Q = Q1 \times Q2, s = (s1, s2) \in Q \text{ and }
    \delta: Q \times \Sigma_1 \mapsto Q \times \Gamma^*_2
    \text{ is the function defined as }
    \delta((q_1, q_2), a) = ((q_1', q_2')), v) \text{ with }
    (q_1',u) = \delta_1(q_1,a)   \text{ and }
    (q_2',v) = \delta_2^*(q_2,u) \text{ and }
    $
    It can be easily verified by induction that
    $f_M = f_{M_2} \circ f_{M_1}$.
\end{proof}

\subsection{FST-Reductions}
% --------------------------------------------------

\begin{definition}[Reduction of Languages]
    \[
        f \colon \Sigma^* \mapsto \Gamma^* \text{ s.t.\ } A = f^{-1}(B)
    \]
    is called a reduction from $A$ to $B$. If such reduction exists, we say $A$ is
    reducable to $B$, denoted by
    \[
        A \reducable B.
    \]
\end{definition}

\begin{theorem}[]\ \\
    If $A \reducable B$ and $B$ is regular, then $A$ is regular. \\
    If $A \reducable B$ and $A$ is not regular, then $B$ is not regular.
\end{theorem}

